Q10

projet.v
@@ -1,5 +1,4 @@
 Require Export Nat.
-Require Export Ltac.
 
 (*Question 1*)
 (*
@@ -29,7 +28,9 @@ Inductive expr : Type :=
 (*Exemple donné à la question 1*)
 Example expr1 : expr := Plus (Cst 1) (Mult (Cst 2) (Cst 3)).
 
-(*exemple : 1 * (2 + 3) * 4 *)
+(*
+exemple : 1 * (2 + 3) * 4 
+*)
 Example expr2 : expr := Mult (Cst 1) (Mult (Plus (Cst 2) (Cst 3)) (Cst 4)).
 
 
@@ -61,6 +62,10 @@ Inductive liste : Type :=
   | lvide : liste
   | ajt : postfix_expr -> liste -> liste.
 
+Notation "pexpr :l: l" := (ajt pexpr l) (right associativity, at level 60).
+
+
+
 
 (*4.2*)
 
@@ -69,32 +74,17 @@ Inductive liste : Type :=
 (*4.3*)
 
 (* 
-1 2 + 3 * 
+1 2 3 * +
 *)
-Example postfix_expr1 := ajt (post_Cst 1) 
-                                (ajt (post_Cst 2) 
-                                     (ajt post_Plus 
-                                          (ajt (post_Cst 3) 
-                                               (ajt post_Mult lvide)
-                                          )
-                                     )
-                                ).
+
+Example postfix_expr1 := (post_Cst 1) :l: (post_Cst 2) :l: (post_Cst 3) :l: post_Mult :l: post_Plus :l: lvide.
 
 (* 
 1 2 3 + * 4 *
 *)
-Example postfix_expr2 := ajt (post_Cst 1) 
-                                (ajt (post_Cst 2)
-                                     (ajt (post_Cst 3) 
-                                          (ajt post_Plus 
-                                               (ajt post_Mult 
-                                                    (ajt (post_Cst 4)
-                                                         (ajt post_Mult lvide)
-                                                    )
-                                                )
-                                          )
-                                     )
-                                ).
+
+Example postfix_expr2 := (post_Cst 1) :l: (post_Cst 2) :l: (post_Cst 3) :l: post_Plus :l: 
+                         post_Mult :l: (post_Cst 4) :l: post_Mult :l: lvide.
 
 (*Question 5*)
 
@@ -103,18 +93,122 @@ Example postfix_expr2 := ajt (post_Cst 1)
 Fixpoint append (l1 l2 : liste) : liste :=
   match l1 with
   |lvide => l2
-  |ajt elt l => ajt elt (append l l2)
+  |ajt elt_2 l_2 => ajt elt_2 (append l_2 l2)
   end.
 
 Notation "l1 @ l2" := (append l1 l2) (right associativity, at level 60).
 
-Example associativity : lvide @ ( postfix_expr1 @ postfix_expr2) = (lvide @ postfix_expr1) @ postfix_expr2.
-Abort.
-Theorem associativity : forall l:liste,
-lvide @ ( postfix_expr1 @ postfix_expr2) = (lvide @ postfix_expr1) @ postfix_expr2.
+Compute postfix_expr1 @ postfix_expr2.
 
-About intro.
+(*5.2*)
 
-Proof
-  intro.
+Lemma associativity : lvide @ (postfix_expr1 @ postfix_expr2) = (lvide @ postfix_expr1) @ postfix_expr2.
+
+Proof.
+  simpl.
+  reflexivity.
+Qed.
+
+(*Question 6*)
+
+Fixpoint translate (e : expr) : liste :=
+  match e with
+  |Cst n => (post_Cst n) :l: lvide
+  |Mult e1 e2 => (translate e1) @ (translate e2) @ post_Mult :l: lvide
+  |Plus e1 e2 => (translate e1) @ (translate e2) @ post_Plus :l: lvide
+  end.
+
+Example test : translate expr1 = postfix_expr1.
+Proof.
+  simpl.
+  reflexivity.
+Qed.
+
+(*Question 7*)
+
+(*7.1*)
+Inductive well_formed : liste -> Prop :=
+| w_cst : forall n, well_formed(n :l: lvide)
+| w_plus : forall l1 l2, well_formed l1 -> well_formed l2 -> well_formed ( l1 @ l2 @ post_Mult :l: lvide)
+| w_fois : forall l1 l2, well_formed l1 -> well_formed l2 -> well_formed ( l1 @ l2 @ post_Plus :l: lvide). 
+
+Compute well_formed postfix_expr1.
+
+(*7.2*)
+
+Lemma wf_ok : forall e : expr, well_formed (translate e).
+Proof.
+  intros e.
+  induction e.
+  - simpl. constructor.
+  - simpl. constructor; assumption.
+  - simpl. constructor; assumption.
+Qed.
+
+(*Question 8*)
+
+(*8.1*)
+
+Inductive pile : Type := 
+  | pvide : pile
+  | empiler : pile -> nat -> pile.
+
+(*8.2*)
+
+Definition sommet (p : pile) : nat := 
+  match p with
+  |pvide => (0-1)
+  |empiler _ n => n
+  end.
+
+Definition depiler (p : pile) : pile := 
+  match p with
+  |pvide => pvide
+  |empiler p n => p
+  end.
+
+Definition show (p : pile) : pile := 
+  p.
+
+Notation "p :p: elt" := (empiler p elt) (left associativity, at level 40).
+
+
+Example test_pile := pvide :p: 1 :p: 2 :p: 3.
+
+Compute show test_pile.
+Compute sommet test_pile.
+Compute depiler test_pile.
+Compute depiler (depiler test_pile).
+Compute depiler (depiler (depiler test_pile)).
+
+(*Question 9*)
+
+(*9.1*)
+
+Fixpoint eval_postfixe (pf_liste : liste) (p : pile) : pile := 
+  match pf_liste with
+  |lvide => p
+  |ajt exp l => match exp with
+                 |post_Cst n => eval_postfixe l (p :p: n)
+                 |post_Mult => eval_postfixe l (depiler (depiler p) :p: ((sommet p) * (sommet (depiler p))))
+                 |post_Plus => eval_postfixe l (depiler (depiler p) :p: ((sommet p) + (sommet (depiler p))))
+                end
+  end.
+
+(*9.2*)
+
+Compute sommet (eval_postfixe postfix_expr1 pvide). (*7*)
+Compute sommet (eval_postfixe postfix_expr2 pvide). (*20*)
+
+Compute sommet (eval_postfixe (postfix_expr2 @ postfix_expr1 @ post_Plus :l: lvide)  pvide). (*27*)
+Compute sommet (eval_postfixe (postfix_expr2 @ postfix_expr1 @ post_Mult :l: lvide)  pvide). (*140*)
+
+(*Question 10*)
+
+(*10.1*)
+
+Lemma append_eval : forall ( e f: liste), forall ( p: pile),
+eval_postfixe (append e f) p = eval_postfixe f (eval_postfixe e p).
+
+
 
